begin on envconcat

theories/Inert.v
@@ -1,4 +1,29 @@
+From Hammer Require Import Tactics.
 Variant inertness : Set :=
   | Inert
   | Jumpy.
 Hint Constructors inertness : core.
+
+Definition i_leq i1 i2 :=
+  match i1, i2 with
+  | Inert, i => True
+  | Jumpy , Jumpy => True
+  | Jumpy , Inert => False
+  end.
+Hint Unfold i_leq : i1 i2.
+
+Definition i_ub i1 i2 i3 :=
+  (i1 = Jumpy \/ i2 = Jumpy) -> i3 = Jumpy.
+Hint Unfold i_ub : i1 i2 i3.
+
+(* if p, then i can be inert.*)
+Definition inert_guard (p : Prop) (i : inertness) : Prop :=
+  ~p -> i = Jumpy.
+
+Theorem i_ub_is_ub : forall i1 i2 i3,
+  i_ub i1 i2 i3 ->
+  i_leq i1 i3 /\ i_leq i2 i3.
+Proof.
+intros.
+destruct i1; destruct i2; destruct i3; sfirstorder.
+Qed.
